exploration

tree/global.v
@@ -31,6 +31,22 @@ Inductive coseqIn: part -> coseq part -> Prop :=
   | CoInSplit1 x xs y ys: force xs = cocons y ys -> x = y  -> coseqIn x xs
   | CoInSplit2 x xs y ys: force xs = cocons y ys -> x <> y -> coseqIn x ys -> coseqIn x xs.
 
+Fixpoint gLparts (p: part) (l: list (option(sort*gtt))): Prop :=
+  match l with
+    | Datatypes.Some(s,g) :: xs => coseqIn p (gparts g) /\ gLparts p xs
+    | Datatypes.None :: xs      => gLparts p xs
+    | nil                       => True
+  end.
+
+Inductive wfg (R: gtt -> Prop): gtt -> Prop :=
+  | wfg_end : wfg R gtt_end
+  | wfg_send: forall p q lis,
+              SList lis ->
+              Forall (fun u => u = Datatypes.None \/ (exists s g, u = Datatypes.Some (s,g) /\ R g)) lis ->
+              wfg R (gtt_send p q lis).
+
+Definition wfgC (g: gtt) := paco1 wfg bot1 g.
+
 (*
 Inductive gt2gtt (R: global -> gtt -> Prop): global -> gtt -> Prop :=
   | gt2gtt_end: gt2gtt R g_end gtt_end
@@ -90,7 +106,8 @@ Fixpoint ounzip2 (l: list (option(sort*gtt))): list gtt :=
 Inductive gttstep (R: gtt -> gtt -> part -> part -> Prop): gtt -> gtt -> part -> part -> Prop :=
   | steq : forall p q l xs s gc,
                   p <> q ->
-                  Datatypes.Some (s, gc) = findpathGI xs l -> gttstep R (gtt_send p q xs) gc p q
+                  Datatypes.Some (s, gc) = findpathGI xs l ->
+                  gttstep R (gtt_send p q xs) gc p q
   | stneq: forall p q r s xs ys,
                   p <> q ->
                   r <> s ->
@@ -133,6 +150,47 @@ Fixpoint wfProj (r: part) (R: gtt -> part -> ltt -> Prop) (l1: list (option(sort
     | _                                                        => False
   end.
 
+Check injective2.
+
+Definition injection3 (R: gtt -> part -> ltt -> Prop) := forall a b c d, R a b c -> R a b d -> c = d.
+
+Lemma wps: forall l1 l2 l3 p R, 
+  injection3 R ->
+  wfProj p R l1 l2 ->
+  wfProj p R l1 l3 -> l2 = l3.
+Proof. intro l1.
+       induction l1; intros.
+       - case_eq l2; case_eq l3; intros.
+         + easy.
+         + subst. simpl in H0. easy.
+         + subst. simpl in H. easy.
+         + subst. simpl in H. easy.
+       - case_eq l2; case_eq l3; intros.
+         + easy.
+         + subst. simpl in H. destruct a. destruct p0. easy.
+           easy.
+         + subst.  simpl in H0. destruct a. destruct p0. easy.
+           easy.
+         + subst. simpl in H1, H0.
+           destruct a. destruct o, o0.
+           destruct p0, p1, p2.
+           simpl.
+           pose proof H as HH.
+           specialize(H g p l2 l3).
+           rewrite H; try easy.
+           destruct H0 as (H0a,(H0b,H0c)).
+           destruct H1 as (H1a,(H1b,H1c)).
+           subst. f_equal. 
+           apply IHl1 with (p := p) (R := R); easy. 
+           destruct p0. easy.
+           destruct p0. easy.
+           destruct p0. easy.
+           destruct o, o0.
+           easy. easy. easy.
+           f_equal.
+           apply IHl1 with (p := p) (R := R); easy. 
+Qed.
+
 Inductive projection (R: gtt -> part -> ltt -> Prop): gtt -> part -> ltt -> Prop :=
   | proj_end : forall g r, (coseqIn r (gparts g) -> False) -> projection R g r (ltt_end)
   | proj_in  : forall p r xs ys,
@@ -153,6 +211,331 @@ Inductive projection (R: gtt -> part -> ltt -> Prop): gtt -> part -> ltt -> Prop
                projection R (gtt_send p q xs) r t.
 
 Definition projectionC g r t := paco3 projection bot3 g r t.
+
+Axiom injup: injection3 (upaco3 projection bot3).
+
+Lemma help: forall xs ys s p,
+            (gLparts p xs -> False) ->
+            wfProj p (upaco3 projection bot3) xs ys ->
+            allSame ys ->
+            In (Datatypes.Some (s, ltt_end)) ys.
+Proof. intro xs.
+       induction xs; intros.
+       - simpl in H. easy.
+       - case_eq ys; intros.
+         + subst. simpl in H0.
+           destruct a. destruct p0. easy.
+           easy.
+         + subst.
+           simpl in H0.
+           destruct a, o. destruct p0, p1.
+           simpl. right.
+           apply IHxs with (p := p).
+           intro Hn. apply H.
+           admit.
+           easy.
+           simpl in H1. admit.
+           destruct p0. easy.
+           easy.
+           simpl.
+           simpl in H1.
+           right.
+           apply IHxs with (p := p).
+           intro Hn. apply H. admit.
+           easy. easy.
+Admitted.
+
+ Lemma projI_same: forall g l1 l2 p,
+ wfgC g -> 
+ wfC l1 ->
+ wfC l2 -> 
+ projectionC g p l1 ->
+ projectionC g p l2 -> l1 = l2.
+Proof. intros.
+       case_eq g; intros.
+       - subst.
+         pinversion H2. subst.
+         pinversion H3. subst.
+         easy.
+         admit.
+         admit.
+       - subst.
+         pinversion H2. subst.
+         pinversion H3. subst.
+         easy.
+         subst.
+         contradiction H4. admit.
+         subst.
+         contradiction H4. admit.
+         subst.
+         admit.
+         admit.
+         subst.
+         pinversion H3. subst.
+         contradiction H4. admit.
+         subst. 
+         specialize(wps l ys ys0 p (upaco3 projection bot3) injup H10 H12); intro Hwps.
+         subst. easy.
+         subst. 
+         specialize(wps l ys ys0 p (upaco3 projection bot3) injup H10 H12); intro Hwps.
+         subst. easy.
+         subst.
+         easy.
+         admit.
+         subst.
+         pinversion H3. subst.
+         contradiction H4. admit.
+         subst.
+         specialize(wps l ys ys0 p (upaco3 projection bot3) injup H10 H12); intro Hwps.
+         subst. easy.
+         subst.
+         specialize(wps l ys ys0 p (upaco3 projection bot3) injup H10 H12); intro Hwps.
+         subst. easy.
+         subst. easy.
+         admit.
+         subst. 
+         pinversion H3. subst. 
+         admit. (*helper*)
+         subst. easy.
+         subst. easy.
+         subst.
+         specialize(wps l ys ys0 p (upaco3 projection bot3) injup H13 H19); intro Hwps.
+         subst. 
+         admit. (*a fact*)
+         admit.
+         admit.
+Admitted.
+
+
+Lemma projL_same: forall l1 l2 l3 p,
+ wfProj p (upaco3 projection bot3) l1 l2 ->
+ wfProj p (upaco3 projection bot3) l1 l3 -> l2 = l3.
+Proof. intro l1.
+       induction l1; intros.
+       - case_eq l2; case_eq l3; intros.
+         + subst. easy.
+         + subst. simpl in H0. easy.
+         + subst. simpl in H. easy.
+         + subst. simpl in H. easy.
+       - case_eq l2; case_eq l3; intros.
+         + easy.
+         + subst. simpl in H. destruct a. destruct p0. easy.
+           easy.
+         + subst. simpl in H0. destruct a. destruct p0. easy.
+           easy.
+         + subst.
+           simpl in H. simpl in H0.
+           destruct a. destruct p0, o, o0. destruct p0, p1.
+           f_equal. 
+           destruct H as (Ha,(Hb,Hc)).
+           destruct H0 as (H0a,(H0b,H0c)). 
+           f_equal. subst. f_equal.
+           specialize(injup g p l3 l2 Hb H0b); easy.
+
+           apply IHl1 with (p := p).
+           easy. easy.
+           easy. easy. easy.
+           destruct o, o0. easy. easy. easy.
+           f_equal. 
+           apply IHl1 with (p := p). easy. easy.
+Qed.
+
+Lemma _319_1: forall p q S T G G' L1 L2,
+  wfC L1 ->
+  wfC L2 ->
+  wfC T ->
+  wfgC G ->
+  wfgC G' ->
+  projectionC G p L1 ->
+  subtypeC (ltt_send q [Datatypes.Some(S,T)]) L1 ->
+  gttstepC G G' p q ->
+  projectionC G' p L2 ->
+  subtypeC T L2.
+Proof. intros p q S T G G' L1 L2 Hwk1 Hwl2 Hwt Hwg Hwg' Hpg Hsl1 Hsg Hpg'.
+       pinversion Hsl1. subst.
+       pinversion Hpg. subst.
+       pinversion Hsg. subst.
+       case_eq xs; intros; subst.
+       - pinversion Hwg.
+         subst. simpl in H1. easy.
+         admit.
+       - case_eq ys; intros; subst.
+         simpl in H5. destruct o. destruct p0. easy.
+         simpl in H2. easy.
+       simpl in H2.
+       destruct o0. destruct p0.
+       destruct o.
+       simpl in H5. destruct p0.
+       case_eq l; intros.
+       - subst. simpl in H9. inversion H9. subst. clear H9.
+         pinversion Hpg'. subst.
+         case_eq T; intros.
+         subst. pfold. constructor.
+         subst. 
+         destruct H2 as (H2a,(H2b,H2c)).
+         destruct H2b as [H2b | H2b].
+         pinversion H2b. subst.
+         destruct H5 as (H5a,(H5b,H5c)).
+         destruct H5b as [H5b | H5b].
+         pinversion H5b. subst.
+         contradict H.
+         case_eq xs; intros; subst.
+         pinversion Hwg'. simpl in H1. easy.
+         admit. admit.
+
+         subst.
+         admit. (*merge case*)
+         admit.
+         easy.
+         admit.
+         easy.
+         
+         subst.
+         destruct H2 as (H2a,(H2b,H2c)).
+         destruct H2b as [H2b | H2b].
+         pinversion H2b. subst.
+         destruct H5 as (H5a,(H5b,H5c)).
+         destruct H5b as [H5b | H5b].
+         pinversion H5b. subst.
+         contradict H. admit.
+         
+         subst.
+         admit. (*merge case*)
+         admit.
+         easy.
+         admit.
+         easy.
+
+         case_eq T; intros. subst.
+         destruct H2 as (H2a,(H2b,H2c)).
+         destruct H2b as [H2b | H2b].
+         pinversion H2b. subst.
+         destruct H5 as (H5a,(H5b,H5c)).
+         destruct H5b as [H5b | H5b].
+         pinversion H5b. subst.
+         contradict H. admit.
+         
+         subst.
+         admit. (*merge case*)
+         admit.
+         easy.
+         admit.
+         easy.
+         
+         subst.
+         destruct H2 as (H2a,(H2b,H2c)).
+         destruct H2b as [H2b | H2b].
+         pinversion H2b. subst.
+         destruct H5 as (H5a,(H5b,H5c)).
+         destruct H5b as [H5b | H5b].
+         pinversion H5b. subst.
+         pfold. constructor.
+         admit. (* issue solved here *)
+         
+         subst. easy.
+         admit.
+         easy.
+         admit.
+         easy.
+         
+         subst.
+         destruct H2 as (H2a,(H2b,H2c)).
+         destruct H2b as [H2b | H2b].
+         pinversion H2b. subst.
+         destruct H5 as (H5a,(H5b,H5c)).
+         destruct H5b as [H5b | H5b].
+         pinversion H5b. subst.
+         easy.
+         subst. easy.
+         admit.
+         subst. easy.
+         admit. easy.
+         
+         subst.
+         case_eq T; intros. subst.
+         destruct H2 as (H2a,(H2b,H2c)).
+         destruct H2b as [H2b | H2b].
+         pinversion H2b. subst.
+         destruct H5 as (H5a,(H5b,H5c)).
+         destruct H5b as [H5b | H5b].
+         pinversion H5b. subst.
+         contradict H1. admit.
+         
+         subst. easy.
+         admit.
+         easy.
+         admit.
+         easy.
+         
+         subst.
+         destruct H2 as (H2a,(H2b,H2c)).
+         destruct H2b as [H2b | H2b].
+         pinversion H2b. subst.
+         destruct H5 as (H5a,(H5b,H5c)).
+         destruct H5b as [H5b | H5b].
+         pinversion H5b. subst. easy.
+
+         subst. easy.
+         admit.
+         easy.
+         admit.
+         easy.
+         
+         subst.
+         destruct H2 as (H2a,(H2b,H2c)).
+         destruct H2b as [H2b | H2b].
+         pinversion H2b. subst.
+         destruct H5 as (H5a,(H5b,H5c)).
+         destruct H5b as [H5b | H5b].
+         pinversion H5b. subst. 
+         pfold. constructor.
+         admit. (* issue solved here *)
+         
+         subst.
+         easy.
+         admit.
+         easy. 
+         admit. 
+         easy.
+         
+         
+         subst.
+         destruct H5 as (H5a,(H5b,H5c)).
+         destruct H5b as [H5b | H5b].
+         pinversion H5b. subst. 
+         destruct H2 as (H2a,(H2b,H2c)).
+         destruct H2b as [H2b | H2b].
+         pinversion H2b. subst.
+         admit. (*helper*)
+         admit.
+         easy.
+         subst.
+         destruct H2 as (H2a,(H2b,H2c)).
+         destruct H2b as [H2b | H2b].
+         pinversion H2b. subst.
+         easy. admit.
+         easy. subst. easy. subst.
+         admit.
+         admit.
+         easy.
+         admit.
+         subst.
+         subst.
+         
+         admit.
+         
+         subst. 
+         simpl in H5. easy.
+         easy. subst. easy.
+         admit. subst.
+         
+         pinversion Hsg.
+         subst. easy. subst.
+         pinversion Hpg'. subst.
+         rewrite Forall_forall in H15.
+         rewrite Forall_forall in H19.
+Admitted.
+
 
 (*
 Definition dropDups {A: Type} (l1 l2: list A) := 
