tree/local.v
@@ -59,7 +59,7 @@ Definition wfC (t: ltt) := paco1 wf bot1 t.
 Fixpoint wfrec (R1: sort -> sort -> Prop) (R2: ltt -> ltt -> Prop) (l1 l2: list (option(sort*ltt))): Prop :=
   match (l1,l2) with
     | (Datatypes.None::xs, Datatypes.None::ys)               => wfrec R1 R2 xs ys
-    | (Datatypes.Some (s,t)::xs, Datatypes.Some (s',t')::ys) => R1 s' s /\ R2 t t' /\ wfrec R1 R2 xs ys
+    | (Datatypes.Some (s',t')::xs, Datatypes.Some (s,t)::ys) => R1 s' s /\ R2 t t' /\ wfrec R1 R2 xs ys
     | (nil, _)                                               => True
     | _                                                      => False
   end.
@@ -67,7 +67,7 @@ Fixpoint wfrec (R1: sort -> sort -> Prop) (R2: ltt -> ltt -> Prop) (l1 l2: list 
 Fixpoint wfsend (R1: sort -> sort -> Prop) (R2: ltt -> ltt -> Prop) (l1 l2: list (option(sort*ltt))): Prop :=
   match (l1,l2) with
     | (Datatypes.None::xs, Datatypes.None::ys)               => wfsend R1 R2 xs ys
-    | (Datatypes.Some (s',t')::xs, Datatypes.Some (s,t)::ys) => R1 s s' /\ R2 t t' /\ wfsend R1 R2 xs ys
+    | (Datatypes.Some (s,t)::xs, Datatypes.Some (s',t')::ys) => R1 s s' /\ R2 t t' /\ wfsend R1 R2 xs ys
     | (nil, _)                                               => True
     | _                                                      => False
   end.
